James C - added output, threaded it through all steps

AssemblyLanguage.thy
@@ -6,27 +6,31 @@ datatype assembly =
   AAssm int
 | CAssm "register set" computation
 | JAssm "comparison set" code_label
+| PAssm
 
 type_synonym assembly_program = "code_label \<rightharpoonup> assembly list"
 
-type_synonym assembly_state = "memory \<times> int option \<times> int \<times> assembly list" (* \<mu>, a, d, \<pi> *)
+type_synonym assembly_state = "memory \<times> int option \<times> int \<times> assembly list \<times> output" 
+  (* \<mu>, a, d, \<pi>, \<omega> *)
 
 fun eval_assembly :: "assembly_program \<Rightarrow> assembly_state \<Rightarrow> assembly_state option" where
-  "eval_assembly \<Pi> (\<mu>, a, d, []) = None"
-| "eval_assembly \<Pi> (\<mu>, a, d, AAssm x # \<pi>) = Some (\<mu>, Some x, d, \<pi>)"
-| "eval_assembly \<Pi> (\<mu>, Some a, d, CAssm dst cmp # \<pi>) = (
+  "eval_assembly \<Pi> (\<mu>, a, d, [], \<omega>) = None"
+| "eval_assembly \<Pi> (\<mu>, a, d, AAssm x # \<pi>, \<omega>) = Some (\<mu>, Some x, d, \<pi>, \<omega>)"
+| "eval_assembly \<Pi> (\<mu>, Some a, d, CAssm dst cmp # \<pi>, \<omega>) = (
     let n = compute cmp (\<mu> a) a d
     in Some (
       if M \<in> dst then \<mu>(a := n) else \<mu>, 
       Some (if A \<in> dst then n else a), 
       if D \<in> dst then n else d, 
-      \<pi>))"
-| "eval_assembly \<Pi> (\<mu>, None, d, CAssm dst cmp # \<pi>) = None"
-| "eval_assembly \<Pi> (\<mu>, a, d, JAssm jmp s # \<pi>) = (
+      \<pi>,
+      \<omega>))"
+| "eval_assembly \<Pi> (\<mu>, None, d, CAssm dst cmp # \<pi>, \<omega>) = None"
+| "eval_assembly \<Pi> (\<mu>, a, d, JAssm jmp s # \<pi>, \<omega>) = (
     if should_jump d jmp
     then case \<Pi> s of 
-        Some \<pi>' \<Rightarrow> Some (\<mu>, None, d, \<pi>')
+        Some \<pi>' \<Rightarrow> Some (\<mu>, None, d, \<pi>', \<omega>)
       | None \<Rightarrow> None
-    else Some (\<mu>, None, d, \<pi>))"
+    else Some (\<mu>, None, d, \<pi>, \<omega>))"
+| "eval_assembly \<Pi> (\<mu>, a, d, PAssm # \<pi>, \<omega>) = Some (\<mu>, a, d, \<pi>, d # \<omega>)"
 
 end
