MachineLanguage.thy
@@ -5,24 +5,27 @@ begin
 datatype machine_instruction =
   AInstr int
 | CInstr "register set" computation "comparison set"
+| PInstr
 
 type_synonym machine_program = "machine_instruction list"
 
-type_synonym machine_state = "memory \<times> int \<times> int \<times> nat" (* \<mu>, a, d, pc *)
+type_synonym machine_state = "memory \<times> int \<times> int \<times> nat \<times> output" (* \<mu>, a, d, pc, \<omega> *)
 
 fun eval_instruction :: "machine_instruction \<Rightarrow> machine_state \<Rightarrow> machine_state" where
-  "eval_instruction (AInstr x) (\<mu>, a, d, pc) = (\<mu>, x, d, Suc pc)"
-| "eval_instruction (CInstr dst cmp jmp) (\<mu>, a, d, pc) = (
+  "eval_instruction (AInstr x) (\<mu>, a, d, pc, \<omega>) = (\<mu>, x, d, Suc pc, \<omega>)"
+| "eval_instruction (CInstr dst cmp jmp) (\<mu>, a, d, pc, \<omega>) = (
     let n = compute cmp (\<mu> a) a d
     in (if M \<in> dst then \<mu>(a := n) else \<mu>, 
         if A \<in> dst then n else a, 
         if D \<in> dst then n else d, 
-        if should_jump n jmp then nat a else Suc pc))"
+        if should_jump n jmp then nat a else Suc pc,
+        \<omega>))"
+| "eval_instruction PInstr (\<mu>, a, d, pc, \<omega>) = (\<mu>, a, d, Suc pc, d # \<omega>)"
 
 fun eval_machine :: "machine_program \<Rightarrow> machine_state \<Rightarrow> machine_state option" where
-  "eval_machine \<Pi> (\<mu>, a, d, pc) = (
+  "eval_machine \<Pi> (\<mu>, a, d, pc, \<omega>) = (
     if pc < length \<Pi> 
-    then Some (eval_instruction (\<Pi> ! pc) (\<mu>, a, d, pc)) 
+    then Some (eval_instruction (\<Pi> ! pc) (\<mu>, a, d, pc, \<omega>)) 
     else None)"
 
 end
