LinearAssemblyLanguage.thy
@@ -5,22 +5,24 @@ begin
 type_synonym l_assembly_program = "code_label \<leadsto> assembly list"
 
 fun eval_l_assembly :: "l_assembly_program \<Rightarrow> assembly_state \<Rightarrow> assembly_state option" where
-  "eval_l_assembly \<Pi> (\<mu>, a, d, []) = None"
-| "eval_l_assembly \<Pi> (\<mu>, a, d, AAssm x # \<pi>) = Some (\<mu>, Some x, d, \<pi>)"
-| "eval_l_assembly \<Pi> (\<mu>, Some a, d, CAssm dst cmp # \<pi>) = (
+  "eval_l_assembly \<Pi> (\<mu>, a, d, [], \<omega>) = None"
+| "eval_l_assembly \<Pi> (\<mu>, a, d, AAssm x # \<pi>, \<omega>) = Some (\<mu>, Some x, d, \<pi>, \<omega>)"
+| "eval_l_assembly \<Pi> (\<mu>, Some a, d, CAssm dst cmp # \<pi>, \<omega>) = (
     let n = compute cmp (\<mu> a) a d
     in Some (
       if M \<in> dst then \<mu>(a := n) else \<mu>, 
       Some (if A \<in> dst then n else a), 
       if D \<in> dst then n else d, 
-      \<pi>))"
-| "eval_l_assembly \<Pi> (\<mu>, None, d, CAssm dst cmp # \<pi>) = None"
-| "eval_l_assembly \<Pi> (\<mu>, a, d, JAssm jmp s # \<pi>) = (
+      \<pi>, 
+      \<omega>))"
+| "eval_l_assembly \<Pi> (\<mu>, None, d, CAssm dst cmp # \<pi>, \<omega>) = None"
+| "eval_l_assembly \<Pi> (\<mu>, a, d, JAssm jmp s # \<pi>, \<omega>) = (
     if should_jump d jmp
     then case lookup \<Pi> s of 
-        Some \<pi>' \<Rightarrow> Some (\<mu>, None, d, \<pi>')
+        Some \<pi>' \<Rightarrow> Some (\<mu>, None, d, \<pi>', \<omega>)
       | None \<Rightarrow> None
-    else Some (\<mu>, None, d, \<pi>))"
+    else Some (\<mu>, None, d, \<pi>, \<omega>))"
+| "eval_l_assembly \<Pi> (\<mu>, a, d, Print # \<pi>, \<omega>) = Some (\<mu>, a, d, \<pi>, d # \<omega>)"
 
 (* linearization correct *)
 
@@ -37,6 +39,8 @@ lemma [simp]: "finite (dom \<Pi>) \<Longrightarrow> eval_assembly \<Pi> \<Sigma>
     from 4(2) show ?case by simp
   next case 5
     thus ?case by auto
+  next case 6
+    thus ?case by simp
   qed 
 
 theorem linearization_correct [simp]: "iterate (eval_assembly \<Pi>) \<Sigma> \<Sigma>' \<Longrightarrow> finite (dom \<Pi>) \<Longrightarrow> 
