StackLanguage.thy
@@ -4,21 +4,23 @@ begin
 
 datatype stack_instruction = 
   Add | Sub | Neg | Eq | Gt | Lt | And | Or | Not
+| Print
 
 type_synonym stack_program = "code_label \<rightharpoonup> stack_instruction list"
 
-type_synonym stack_state = "int list \<times> stack_instruction list" (* \<sigma>, \<pi> *)
+type_synonym stack_state = "int list \<times> stack_instruction list \<times> output" (* \<sigma>, \<pi>, \<omega> *)
 
 fun eval_stack :: "stack_program \<Rightarrow> stack_state \<Rightarrow> stack_state option" where
-  "eval_stack \<Pi> (i1 # i2 # \<sigma>, Add # \<pi>) = Some ((i2 + i1) # \<sigma>, \<pi>)"
-| "eval_stack \<Pi> (i1 # i2 # \<sigma>, Sub # \<pi>) = Some ((i2 - i1) # \<sigma>, \<pi>)"
-| "eval_stack \<Pi> (i1 # \<sigma>, Neg # \<pi>) = Some ((-i1) # \<sigma>, \<pi>)"
-| "eval_stack \<Pi> (i1 # i2 # \<sigma>, Eq # \<pi>) = Some (unboolify (i2 = i1) # \<sigma>, \<pi>)"
-| "eval_stack \<Pi> (i1 # i2 # \<sigma>, Gt # \<pi>) = Some (unboolify (i2 > i1) # \<sigma>, \<pi>)"
-| "eval_stack \<Pi> (i1 # i2 # \<sigma>, Lt # \<pi>) = Some (unboolify (i2 < i1) # \<sigma>, \<pi>)"
-| "eval_stack \<Pi> (i1 # i2 # \<sigma>, And # \<pi>) = Some (unboolify (boolify i2 \<and> boolify i1) # \<sigma>, \<pi>)"
-| "eval_stack \<Pi> (i1 # i2 # \<sigma>, Or # \<pi>) = Some (unboolify (boolify i2 \<or> boolify i1) # \<sigma>, \<pi>)"
-| "eval_stack \<Pi> (i1 # \<sigma>, Not # \<pi>) = Some (unboolify (\<not> boolify i1) # \<sigma>, \<pi>)"
+  "eval_stack \<Pi> (i1 # i2 # \<sigma>, Add # \<pi>, \<omega>) = Some ((i2 + i1) # \<sigma>, \<pi>, \<omega>)"
+| "eval_stack \<Pi> (i1 # i2 # \<sigma>, Sub # \<pi>, \<omega>) = Some ((i2 - i1) # \<sigma>, \<pi>, \<omega>)"
+| "eval_stack \<Pi> (i1 # \<sigma>, Neg # \<pi>, \<omega>) = Some ((-i1) # \<sigma>, \<pi>, \<omega>)"
+| "eval_stack \<Pi> (i1 # i2 # \<sigma>, Eq # \<pi>, \<omega>) = Some (unboolify (i2 = i1) # \<sigma>, \<pi>, \<omega>)"
+| "eval_stack \<Pi> (i1 # i2 # \<sigma>, Gt # \<pi>, \<omega>) = Some (unboolify (i2 > i1) # \<sigma>, \<pi>, \<omega>)"
+| "eval_stack \<Pi> (i1 # i2 # \<sigma>, Lt # \<pi>, \<omega>) = Some (unboolify (i2 < i1) # \<sigma>, \<pi>, \<omega>)"
+| "eval_stack \<Pi> (i1 # i2 # \<sigma>, And # \<pi>, \<omega>) = Some (unboolify (boolify i2 \<and> boolify i1) # \<sigma>, \<pi>, \<omega>)"
+| "eval_stack \<Pi> (i1 # i2 # \<sigma>, Or # \<pi>, \<omega>) = Some (unboolify (boolify i2 \<or> boolify i1) # \<sigma>, \<pi>, \<omega>)"
+| "eval_stack \<Pi> (i1 # \<sigma>, Not # \<pi>, \<omega>) = Some (unboolify (\<not> boolify i1) # \<sigma>, \<pi>, \<omega>)"
+| "eval_stack \<Pi> (i1 # \<sigma>, Print # \<pi>, \<omega>) = Some (\<sigma>, \<pi>, i1 # \<omega>)"
 | "eval_stack \<Pi> \<Sigma> = None"
 
 end
